thys/Untyped_Lambda_Calculus/Translation_ILC_to_LC.thy
@@ -233,5 +233,4 @@ using assms FFVars_tr'  uniform_good by auto
 
 
 
-
 end 
